bring back timeout + match guardchecker with hunting

theories/Inductives.v
@@ -39,23 +39,28 @@ Inductive guard_exc :=
   | NoReductionPossible. 
 
 (*max bind steps *)
-Definition max_steps := 0. 
-(* Definition catchE := @catchE max_steps. 
-Arguments catchE {_ _}.  *)
-Definition catchMap := @catchMap _ TimeoutErr. 
+Definition max_steps := 3000. 
+Definition catchE := @catchE max_steps. 
+Arguments catchE {_ _}. 
+Definition catchMap := @catchMap max_steps guard_exc TimeoutErr. 
 Arguments catchMap {_ _}. 
   
-Instance trace_monad : Monad (@TraceM guard_exc).
-apply trace_monad. exact TimeoutErr.
+Instance: Monad (@TraceM guard_exc).
+Proof.
+  apply trace_monad.
+  all: (apply max_steps || apply TimeoutErr).
 Defined.
 
-(* Notation "'exc' A" := (excOn guard_exc A) (at level 100) : exc_scope.  *)
 Notation "'exc' A" := (@TraceM guard_exc A) (at level 100) : exc_scope. 
-(* Definition unwrap := @exc_unwrap. *)
 Definition unwrap := @trc_unwrap.
 Arguments unwrap { _ _ _ _}. 
 
-Instance: TrcUnwrap list := list_trc_unwrap TimeoutErr.
+
+Instance: TrcUnwrap (Y := guard_exc) list. 
+Proof.
+  apply list_trc_unwrap.
+  all: (apply max_steps || apply TimeoutErr).
+Defined.
 
 Notation "a == b" := (eqb a b) (at level 70) : exc_scope. 
 Notation "a != b" := (negb(a==b)) (at level 90) : exc_scope.
